Add generators for operational semantics.

HoareLogic/SequentialSemantics.v
@@ -1,4 +1,7 @@
 Require Import Coq.Relations.Relation_Operators.
+Require Import Coq.Logic.Classical_Prop.
+Require Import Coq.Logic.Classical_Pred_Type.
+Require Import Logic.lib.NatChoice.
 Require Import Logic.MinimunLogic.LogicBase.
 Require Import Logic.PropositionalLogic.KripkeSemantics.
 Require Import Logic.SeparationLogic.SeparationAlgebra.
@@ -107,7 +110,7 @@ Class NormalBigStepSemantics (P: ProgrammingLanguage) (state: Type) (BSS: BigSte
   access_defined: forall s c, exists ms, access s c ms
 }.
 
-Class NormalSmallStepSemantics (P: ProgrammingLanguage) (state: Type) (BSS: SmallStepSemantics P state): Type := {
+Class NormalSmallStepSemantics (P: ProgrammingLanguage) (state: Type) (SSS: SmallStepSemantics P state): Type := {
   step_defined: forall cs, exists mcs, step cs mcs
 }.
 
@@ -115,21 +118,73 @@ Class NormalSmallStepSemantics (P: ProgrammingLanguage) (state: Type) (BSS: Smal
 (* Generators                                       *)
 (****************************************************)
 
+Definition step' {P: ProgrammingLanguage} {state: Type} {SSSS: SimpleSmallStepSemantics P state} (cs: cmd * state) (mcs: MetaState (cmd * state)) :=
+  match mcs with
+  | Terminating cs0 => simple_step cs cs0
+  | NonTerminating => False
+  | Error => forall cs0, ~ simple_step cs cs0
+  end.
+
 Instance SSS_SimpleSSS {P: ProgrammingLanguage} {state: Type} (SSSS: SimpleSmallStepSemantics P state): SmallStepSemantics P state :=
-  Build_SmallStepSemantics _ _
-   (fun cs mcs =>
-      match mcs with
-      | Terminating cs0 => simple_step cs cs0
-      | NonTerminating => False
-      | Error => forall cs0, ~ simple_step cs cs0
-      end).
+  Build_SmallStepSemantics _ _ step'.
+
+Instance nSSS_SimpleSSS {P: ProgrammingLanguage} {state: Type} (SSSS: SimpleSmallStepSemantics P state): NormalSmallStepSemantics P state (SSS_SimpleSSS SSSS).
+Proof.
+  constructor.
+  intros.
+  destruct (classic (exists cs0, simple_step cs cs0)).
+  + destruct H as [cs0 ?].
+    exists (Terminating cs0).
+    auto.
+  + exists Error.
+    simpl.
+    intros ? ?; apply H; clear H.
+    exists cs0; auto.
+Qed.
+
+Definition access' {P: ProgrammingLanguage} {Imp: ImperativeProgrammingLanguage P} {state: Type} {SSS: SmallStepSemantics P state} (s: state) (c: cmd) (ms: MetaState state) :=
+  
+    match ms with
+    | Terminating s0 => clos_refl_trans _ lift_step (Terminating (c, s))  (Terminating (Sskip, s0))
+    | NonTerminating => clos_refl_trans _ lift_step (Terminating (c, s)) NonTerminating \/ exists cs: nat -> cmd * state, cs 0 = (c, s) /\ forall k, step (cs k) (Terminating (cs (S k)))
+    | Error => clos_refl_trans _ lift_step (Terminating (c, s)) Error
+    end.
 
 Instance BSS_SSS {P: ProgrammingLanguage} {Imp: ImperativeProgrammingLanguage P} {state: Type} (SSS: SmallStepSemantics P state): BigStepSemantics P state :=
-  Build_BigStepSemantics _ _
-   (fun s c ms =>
-      clos_refl_trans _ lift_step (Terminating (c, s))
-        match ms with
-        | Terminating s0 => Terminating (Sskip, s0)
-        | NonTerminating => NonTerminating
-        | Error => Error
-        end).
+  Build_BigStepSemantics _ _ access'.
+
+Instance nBSS_SSS {P: ProgrammingLanguage} {Imp: ImperativeProgrammingLanguage P} {state: Type} (SSS: SmallStepSemantics P state) {nSSS: NormalSmallStepSemantics P state SSS}: NormalBigStepSemantics P state (BSS_SSS SSS).
+Proof.
+  constructor.
+  intros.
+  apply NNPP; intro.
+  pose proof not_ex_all_not _ _ H.
+  pose proof H0 Error.
+  pose proof H0 NonTerminating.
+  pose proof (fun s => H0 (Terminating s)).
+  clear H H0.
+  simpl in H1, H2, H3.
+  apply not_or_and in H2; destruct H2.
+  apply H0.
+  apply (nat_coinduction
+          (fun cs => clos_refl_trans _ lift_step
+                       (Terminating (c, s)) (Terminating cs))
+          (fun cs1 cs2 => step cs1 (Terminating cs2))).
+  + apply rt_refl.
+  + intros [c0 s0] ?.
+    destruct (step_defined (c0, s0)) as [mcs ?].
+    destruct mcs as [| | [c1 s1]].
+    - exfalso; apply H1.
+      apply rt_trans with (Terminating (c0, s0)); auto.
+      apply rt_step.
+      constructor; auto.
+    - exfalso; apply H.
+      apply rt_trans with (Terminating (c0, s0)); auto.
+      apply rt_step.
+      constructor; auto.
+    - exists (c1, s1).
+      split; auto.
+      apply rt_trans with (Terminating (c0, s0)); auto.
+      apply rt_step.
+      constructor; auto.
+Qed.
